Add type substitution

Defs.thy
@@ -16,6 +16,7 @@ nominal_datatype "term" =
  | Lam x::"var" "\<tau>" e::"term" binds x in e  ("\<lambda> _ : _ . _" 50)
  | TyLam a::"tyvar" e::"term" binds a in e ("\<Lambda> _ . _" 50)
  | App "term" "term"
+ | TyApp "term" "\<tau>"
  | Unit
  | Let x::"var" "term" e2::"term" binds x in e2
 
@@ -26,15 +27,15 @@ declare term.fv_defs[simp]
 lemma no_vars_in_ty[simp]: "atom (x :: var) \<sharp> (ty :: \<tau>)"
   by (induction ty rule: \<tau>.induct) auto
 
-(*nominal_function isin :: "var * \<tau> \<Rightarrow> \<Gamma> \<Rightarrow> bool" (infixr "\<in>" 80) where
+nominal_function isin :: "var * \<tau> \<Rightarrow> \<Gamma> \<Rightarrow> bool" (infixr "\<in>" 80) where
   "isin _ [] = False"
 | "isin (x, t) ((y, t')#xs) = (if x = y then t = t' else isin (x, t) xs)"
        apply (all_trivials)
       apply (simp add: eqvt_def isin_graph_aux_def)
-     apply (metis list.exhaust old.prod.exhaust)
+     apply (metis list.exhaust prod.exhaust)
     apply simp
   done
-nominal_termination (eqvt) by lexicographic_order*)
+nominal_termination (eqvt) by lexicographic_order
 
 (** subrules *)
 nominal_function
@@ -44,6 +45,7 @@ where
 | "is_value (\<lambda> x : \<tau> . e) = True"
 | "is_value (\<Lambda> a . e) = True"
 | "is_value (App e1 e2) = False"
+| "is_value (TyApp e \<tau>) = False"
 | "is_value Unit = True"
 | "is_value (Let x e1 e2) = False"
   apply (auto simp: eqvt_def is_value_graph_aux_def)
@@ -90,24 +92,25 @@ proof -
 qed
 
 (** substitutions *)
-nominal_function
-subst_term :: "term => var => term => term"
+nominal_function subst_term :: "term => var => term => term"
 where
 "subst_term e x (Var y) = (if x=y then e else Var y)"
 | "atom y \<sharp> (x, e) \<Longrightarrow> subst_term e x (\<lambda> y : \<tau> . e2) = (Lam y \<tau> (subst_term e x e2))"
 | "atom y \<sharp> (x, e) \<Longrightarrow> subst_term e x (\<Lambda> y . e2) = (\<Lambda> y . subst_term e x e2)"
 | "subst_term e x (App e1 e2) = (App (subst_term e x e1) (subst_term e x e2))"
+| "subst_term e x (TyApp e1 \<tau>) = (TyApp (subst_term e x e1) \<tau>)"
 | "subst_term _ _ Unit = Unit"
 | "atom y \<sharp> (x, e) \<Longrightarrow> subst_term e x (Let y e1 e2) = (Let y (subst_term e x e1) (subst_term e x e2))"
 proof goal_cases
+next
   case (3 P x)
   then obtain e y t where P: "x = (e, y, t)" by (metis prod.exhaust)
   then show ?case
     apply (cases t rule: term.strong_exhaust[of _ _ "(y, e)"])
          apply (auto simp: 3)
-    using 3(2) 3(3) 3(6) P fresh_star_def by blast+
+    using 3(2) 3(3) 3(7) P fresh_star_def by blast+
 next
-  case (10 y x e \<tau> e2 y' x' e' \<tau>' e2')
+  case (11 y x e \<tau> e2 y' x' e' \<tau>' e2')
 
   obtain c::var where "atom c \<sharp> (y, y',  e, x, e', x', e2, e2', subst_term_sumC (e, x, e2), subst_term_sumC (e', x', e2'))" using obtain_fresh by blast
   then have c: "atom c \<sharp> (subst_term_sumC (e, x, e2), x, e)" "atom c \<sharp> (subst_term_sumC (e', x', e2'), x', e')" "atom c \<sharp> (y, e2, y', e2')" using fresh_Pair by fastforce+
@@ -116,14 +119,14 @@ next
   have sort_same_y': "sort_of (atom c) = sort_of (atom y')" by simp
 
   have 1: "(\<lambda> y : \<tau> . subst_term_sumC (e, x, e2)) = (\<lambda> c : \<tau> . subst_term_sumC (e, x, (y \<leftrightarrow> c) \<bullet> e2))"
-    using Abs_lst_rename_deep[OF c(1) 10(5) sort_same_y 10(1)] term.eq_iff(2) by blast
+    using Abs_lst_rename_deep[OF c(1) 11(5) sort_same_y 11(1)] term.eq_iff(2) by blast
   have 2: "(\<lambda> y' : \<tau>' . subst_term_sumC (e', x', e2')) = (\<lambda> c : \<tau> . subst_term_sumC (e, x, (y' \<leftrightarrow> c) \<bullet> e2'))"
-    using Abs_lst_rename_deep[OF c(2) 10(6) sort_same_y' 10(2)] term.eq_iff(2) 10(7) by auto
-  have 3: "(y \<leftrightarrow> c) \<bullet> e2 = (y' \<leftrightarrow> c) \<bullet> e2'" using Abs_lst_rename_both[OF c(3) sort_same_y sort_same_y'] 10(7) by force
+    using Abs_lst_rename_deep[OF c(2) 11(6) sort_same_y' 11(2)] term.eq_iff(2) 11(7) by auto
+  have 3: "(y \<leftrightarrow> c) \<bullet> e2 = (y' \<leftrightarrow> c) \<bullet> e2'" using Abs_lst_rename_both[OF c(3) sort_same_y sort_same_y'] 11(7) by force
 
   show ?case using 1 2 3 by argo
 next
-  case (15 y x e e2 y' x' e' e2')
+  case (17 y x e e2 y' x' e' e2')
   
   obtain c::tyvar where "atom c \<sharp> (y, y',  e, x, e', x', e2, e2', subst_term_sumC (e, x, e2), subst_term_sumC (e', x', e2'))" using obtain_fresh by blast
   then have c: "atom c \<sharp> (subst_term_sumC (e, x, e2), x, e)" "atom c \<sharp> (subst_term_sumC (e', x', e2'), x', e')" "atom c \<sharp> (y, e2, y', e2')" using fresh_Pair by fastforce+
@@ -132,14 +135,14 @@ next
   have sort_same_y': "sort_of (atom c) = sort_of (atom y')" by simp
 
   have 1: "(\<Lambda> y . subst_term_sumC (e, x, e2)) = (\<Lambda> c . subst_term_sumC (e, x, (y \<leftrightarrow> c) \<bullet> e2))"
-    using Abs_lst_rename_deep[OF c(1) 15(5) sort_same_y 15(1)] term.eq_iff(3) by presburger
+    using Abs_lst_rename_deep[OF c(1) 17(5) sort_same_y 17(1)] term.eq_iff(3) by presburger
   have 2: "(\<Lambda> y' . subst_term_sumC (e', x', e2')) = (\<Lambda> c . subst_term_sumC (e, x, (y' \<leftrightarrow> c) \<bullet> e2'))"
-    using Abs_lst_rename_deep[OF c(2) 15(6) sort_same_y' 15(2)] term.eq_iff(3) 15(7) by auto
-  have 3: "(y \<leftrightarrow> c) \<bullet> e2 = (y' \<leftrightarrow> c) \<bullet> e2'" using Abs_lst_rename_both[OF c(3) sort_same_y sort_same_y'] 15(7) by force
+    using Abs_lst_rename_deep[OF c(2) 17(6) sort_same_y' 17(2)] term.eq_iff(3) 17(7) by auto
+  have 3: "(y \<leftrightarrow> c) \<bullet> e2 = (y' \<leftrightarrow> c) \<bullet> e2'" using Abs_lst_rename_both[OF c(3) sort_same_y sort_same_y'] 17(7) by force
 
   show ?case using 1 2 3 by argo
 next
-  case (24 y x e e1 e2 y' x' e' e1' e2')
+  case (31 y x e e1 e2 y' x' e' e1' e2')
 
   obtain c::var where "atom c \<sharp> (y, y',  e, x, e', x', e2, e2', subst_term_sumC (e, x, e2), subst_term_sumC (e', x', e2'))" using obtain_fresh by blast
   then have c: "atom c \<sharp> (subst_term_sumC (e, x, e2), x, e)" "atom c \<sharp> (subst_term_sumC (e', x', e2'), x', e')" "atom c \<sharp> (y, e2, y', e2')" using fresh_Pair by fastforce+
@@ -149,15 +152,48 @@ next
 
   let ?e1 = "subst_term_sumC (e, x, e1)"
   let ?e1' = "subst_term_sumC (e', x', e1')"
-  have 0: "?e1 = ?e1'" using 24 by simp
+  have 0: "?e1 = ?e1'" using 31 by simp
   have 1: "Let y ?e1 (subst_term_sumC (e, x, e2)) = Let c ?e1 (subst_term_sumC (e, x, (y \<leftrightarrow> c) \<bullet> e2))"
-    using Abs_lst_rename_deep[OF c(1) 24(9) sort_same_y 24(2)] 0 term.eq_iff(6) by blast
+    using Abs_lst_rename_deep[OF c(1) 31(9) sort_same_y 31(2)] 0 term.eq_iff(6) by fastforce
   have 2: "Let y' ?e1' (subst_term_sumC (e', x', e2')) = Let c ?e1 (subst_term_sumC (e, x, (y' \<leftrightarrow> c) \<bullet> e2'))"
-    using Abs_lst_rename_deep[OF c(2) 24(10) sort_same_y' 24(4)] 0 term.eq_iff(6) 24(11) by auto
-  have 3: "(y \<leftrightarrow> c) \<bullet> e2 = (y' \<leftrightarrow> c) \<bullet> e2'" using Abs_lst_rename_both[OF c(3) sort_same_y sort_same_y'] 24(11) by force
+    using Abs_lst_rename_deep[OF c(2) 31(10) sort_same_y' 31(4)] 0 term.eq_iff(6) 31(11) by auto
+  have 3: "(y \<leftrightarrow> c) \<bullet> e2 = (y' \<leftrightarrow> c) \<bullet> e2'" using Abs_lst_rename_both[OF c(3) sort_same_y sort_same_y'] 31(11) by force
 
   show ?case using 1 2 3 by argo
 qed (auto simp: eqvt_def subst_term_graph_aux_def)
+nominal_termination (eqvt) by lexicographic_order
+
+nominal_function subst_type :: "\<tau> \<Rightarrow> tyvar \<Rightarrow> \<tau> \<Rightarrow> \<tau>" where
+  "subst_type _ _ TyUnit = TyUnit"
+| "subst_type \<tau> a (TyVar b) = (if a=b then \<tau> else TyVar b)"
+| "subst_type \<tau> a (TyArrow \<tau>1 \<tau>2) = TyArrow (subst_type \<tau> a \<tau>1) (subst_type \<tau> a \<tau>2)"
+| "atom b \<sharp> (\<tau>, a) \<Longrightarrow> subst_type \<tau> a (TyForall b \<sigma>) = TyForall b (subst_type \<tau> a \<sigma>)"
+proof goal_cases
+  case (3 P x)
+  then obtain \<tau> a t where P: "x = (\<tau>, a, t)" by (metis prod.exhaust)
+  then show ?case
+    apply (cases t rule: \<tau>.strong_exhaust[of _ _ "(\<tau>, a)"])
+       apply (auto simp: 3)
+    using 3(4) P fresh_star_def by blast
+next
+  case (13 b \<tau> a \<sigma> b' \<tau>' a' \<sigma>')
+
+  obtain c::tyvar where "atom c \<sharp> (b, b', \<tau>, a, \<tau>', a', \<sigma>, \<sigma>', subst_type_sumC (\<tau>, a, \<sigma>), subst_type_sumC (\<tau>', a', \<sigma>'))" using obtain_fresh by blast
+  then have c: "atom c \<sharp> (subst_type_sumC (\<tau>, a, \<sigma>), a, \<tau>)" "atom c \<sharp> (subst_type_sumC (\<tau>', a', \<sigma>'), a', \<tau>')" "atom c \<sharp> (b, \<sigma>, b', \<sigma>')" using fresh_Pair by fastforce+
+
+  have sort_same_b: "sort_of (atom c) = sort_of (atom b)" by simp
+  have sort_same_b': "sort_of (atom c) = sort_of (atom b')" by simp
+
+  from 13 have fresh: "atom b \<sharp> (a, \<tau>)" "atom b' \<sharp> (a', \<tau>')" using fresh_Pair by fastforce+
+
+  have 1: "(\<forall> b . subst_type_sumC (\<tau>, a, \<sigma>)) = (\<forall> c . subst_type_sumC (\<tau>, a, (b \<leftrightarrow> c) \<bullet> \<sigma>))"
+    using Abs_lst_rename_deep[OF c(1) fresh(1) sort_same_b 13(1)] \<tau>.eq_iff(4) by blast
+  have 2: "(\<forall> b' . subst_type_sumC (\<tau>', a', \<sigma>')) = (\<forall> c . subst_type_sumC (\<tau>, a, (b' \<leftrightarrow> c) \<bullet> \<sigma>'))"
+    using Abs_lst_rename_deep[OF c(2) fresh(2) sort_same_b' 13(2)] \<tau>.eq_iff(4) 13(7) by blast
+  have 3: "(b \<leftrightarrow> c) \<bullet> \<sigma> = (b' \<leftrightarrow> c) \<bullet> \<sigma>'" using Abs_lst_rename_both[OF c(3) sort_same_b sort_same_b'] 13(7) by fastforce
+
+  show ?case using 1 2 3 by argo
+qed (auto simp: eqvt_def subst_type_graph_aux_def)
 nominal_termination (eqvt) by lexicographic_order
 
 lemma fresh_subst_term: "\<lbrakk> atom z \<sharp> s ; z = y \<or> atom z \<sharp> t \<rbrakk> \<Longrightarrow> atom z \<sharp> subst_term s y t"
@@ -187,6 +223,8 @@ T_UnitI: "(\<Gamma> \<turnstile> Unit : TyUnit)"
 | T_LetI: "\<lbrakk>atom x \<sharp> (\<Gamma>, e1) ;
 ( ( x ,  \<tau>1 ) # \<Gamma>  \<turnstile> e2 : \<tau>2) ; (\<Gamma> \<turnstile> e1 : \<tau>1)\<rbrakk> \<Longrightarrow>
 (\<Gamma> \<turnstile>  (Let x e1 e2)  : \<tau>2)"
+
+(*| T_InstI: "\<lbrakk> \<Gamma> \<turnstile> e : (\<forall>a . \<sigma>) \<rbrakk> \<Longrightarrow> \<Gamma> \<turnstile> " *)
 
 lemma fresh_not_isin: "atom x \<sharp> \<Gamma> \<Longrightarrow> \<nexists>t'. isin (x, t') \<Gamma>"
   by (induction \<Gamma>) (auto simp: fresh_Pair fresh_Cons fresh_at_base(2))
